found monad structure for pure itree spec and proved monad laws hold on it

theories/Dijkstra/ItreeDijkstra.v
@@ -20,8 +20,8 @@ From ITree Require Import
      Events.MapDefault
      Events.State
      Events.StateFacts
-     Dijkstra.DijkstraMonadExamples
      Core.Divergence
+   (*  Simple *)
 .
 
 From Paco Require Import paco.
@@ -31,35 +31,110 @@ Import MonadNotation.
 Local Open Scope monad_scope.
 Local Open Scope string_scope.
 
+CoFixpoint spin {E: Type -> Type} {A : Type}  : itree E A := Tau spin.
+
+Lemma spin_div : forall E A, @divergence E A spin.
+Proof.
+  intros. pcofix CIH. pfold. unfold divergence_. 
+  cbn. constructor. right. auto.
+Qed.
+
+(*this implies that if a spec w accepts spin, then bind w f should too?   *)
+Lemma spin_bind : forall (E : Type -> Type) (A B : Type) (f : A -> itree E B), spin ≈ bind spin f.
+Proof.
+  intros. pcofix CIH. pfold. unfold bind. simpl. red.
+  cbn. constructor. right. auto.
+Qed.
+
 Inductive Void : Type -> Type := .
 Definition tau_invar (E : Type -> Type) (A : Type) (P : itree E A -> Prop) : Prop :=
     forall (t : itree E A), (P t -> (P (Tau t))) /\(P (Tau t) -> P t).
+(* maybe  *)
+Inductive resp_euttF  {E : Type -> Type} {A : Type} (F : (itree E A -> Prop) -> Prop)  (P : itree E A -> Prop): Prop :=
+  resp_eutt_intro (t1 t2 : itree E A) (Heutt : t1 ≈ t2) (Hiff : P t1 <-> P t2).
 
+Hint Constructors resp_euttF.
+                  
+Definition resp_eutt_ {E A} sim :=
+  fun P => @resp_euttF E A sim P.
+
+Hint Unfold resp_eutt_.
+
+Lemma resp_euttF_mono {E A} sim sim' P (IN : resp_euttF sim P) (LE : sim <1= sim') :
+  @resp_euttF E A sim' P.
+Proof.
+  induction IN; eauto.
+Qed.
+
+Lemma resp_euttF_mono' {E A} : monotone1 (@resp_euttF E A).
+Proof.
+  unfold monotone1. intros.
+  eapply resp_euttF_mono; eauto.
+Qed.
+
+Hint Resolve resp_euttF_mono' : paco.
+
+Definition resp_eutt' {E A} := paco1 (@resp_euttF E A) bot1.
+
+Definition resp_eutt (E : Type -> Type) (A : Type) (P : itree E A -> Prop) : Prop :=
+  forall (t1 t2 : itree E A), t1 ≈ t2 -> (P t1 <-> P t2).
+
+Lemma tau_invar_resp_eutt1: forall (E : Type -> Type) (A : Type) (P : itree E A -> Prop),
+                                 (forall t1 t2, t1 ≈ t2 ->(P t1 <-> P t2)) -> tau_invar E A P.
+  Proof.
+    intros. unfold tau_invar. split; intros;
+    eapply H; try eassumption; rewrite tau_eutt; reflexivity.
+  Qed.
+(* not sure that did anything
+Lemma tau_invar_resp_eutt2_aux : forall (A : Type) (P : itree Void A -> Prop),
+      tau_invar Void A P -> resp_eutt' P.
+  Proof.
+    intros A P HP. unfold tau_invar in *.
+    pcofix CIH. pfold. 
+    constructor.
+    revert H t1 t2.
+    (*pcofix CIH.
+    split.
+    -*)
+
+  Admitted.
+*)
+Ltac inv_div_ret := match goal with [ H : divergenceF _ (RetF _) |- _  ] => inversion H end.
+Lemma div_ret_eutt : forall (E : Type -> Type) (A : Type) (t: itree E A) (a : A),
+      divergence t -> ~(t ≈ ret a).
+  Proof.
+    intros. intros HContra. rewrite HContra in H. pinversion H.
+  Qed.  
+
+Lemma ret_eutt_div : forall (E : Type -> Type) (A : Type) (t : itree E A) (a : A),
+      t ≈ ret a -> ~ (divergence t).
+  Proof.
+    intros. intros HContra. rewrite H in HContra. pinversion HContra.
+  Qed.
+
+Lemma div_spin_eutt : forall (A : Type) (t : itree Void A), divergence t -> t ≈ spin.
+Proof.
+  intros A. pcofix CIH. intros. pfold. red. cbn.
+  destruct (observe t) eqn : Heqt.
+  - specialize (itree_eta t) as H. rewrite Heqt in H. rewrite H in H0. pinversion H0.
+  - constructor. right. apply CIH. specialize (itree_eta t) as H. rewrite Heqt in H.
+    assert (t ≈ Tau t0).
+    + rewrite H. reflexivity.
+    + rewrite <- tau_eutt. rewrite <- H1. auto.
+  - destruct e.
+Qed.
 
 Section PureITree.
-
-  (*how to deal with nonterminsim*)
-  (* partial correctness itrees   *)
-  (* match t with Ret a => p (inl a)  *)
   
   Definition PureITree A := itree Void A.
 
-  (* can interpretation deal with infinite taus*)
-
-  Definition _PureITreeSpec A := forall (p : itree Void A -> Prop), (tau_invar Void A p) -> Prop.
+  Definition _PureITreeSpec A := forall (p : itree Void A -> Prop), (resp_eutt Void A p) -> Prop.
 
   Definition _retpi A (a : A) : _PureITreeSpec A := fun p _ => p (ret a).
 
-  (*I will axiomatize into existence two functions on itrees and talk to steve about if they are 
-   feasible*)
-  
-  
-
   Definition monotonici A (w : _PureITreeSpec A) :=
-    forall (p p' : itree Void A -> Prop) (Hp : tau_invar Void A p) (Hp' :tau_invar Void A p'),
+    forall (p p' : itree Void A -> Prop) (Hp : resp_eutt Void A p) (Hp' : resp_eutt Void A p'),
                                           (forall i', p i' -> p' i') -> w p Hp -> w p' Hp'. 
-(* need the fact that bind preserves this tau invariance condition*) 
-
 
   Definition PureITreeSpec A := {w : _PureITreeSpec A | monotonici A w}.
 
@@ -68,11 +143,18 @@ Section PureITree.
     unfold monotonici. intuition. unfold _retpi in *. auto.
   Qed.
 
- (* is is_val a decidable prop   *)
   Inductive is_val A (a : A) : itree Void A -> Prop :=
     | base :  is_val A a (ITreeDefinition.Ret a)
     | tau (t : itree Void A): is_val A a t -> is_val A a (Tau t) .
 
+  Definition is_val_eutt A (a : A) (t : itree Void A) := t ≈ ret a.
+
+  Lemma is_val_resp_eutt : forall A a, resp_eutt Void A (is_val_eutt A a).
+    Proof.
+      intros. intros t1 t2. unfold is_val_eutt. split; intros.
+      - rewrite H in H0. auto.
+      - rewrite H. auto.
+    Qed.
 
   Lemma is_val_tau_invar : forall A (a : A), tau_invar Void A (is_val A a).
   Proof.
@@ -80,6 +162,18 @@ Section PureITree.
     - constructor. auto.
     - inversion H. auto.
   Qed.
+
+  Lemma eutt_reta_or_spin_aux : forall A (t : itree Void A), (forall a, ~(t≈ ret a)) -> divergence t.
+    Proof.
+      intros A. pcofix CIH. intros. pfold. unfold divergence_.
+      destruct (observe t) eqn:Heqt.
+      - specialize (itree_eta t) as H. rewrite Heqt in H.
+        specialize (H0 r0). rewrite H in H0. exfalso. apply H0.
+        reflexivity.
+      - specialize (itree_eta t) as H. rewrite Heqt in H. constructor. right. eapply CIH; eauto.
+        intros. rewrite <- tau_eutt. rewrite <- H. auto.
+      - destruct e.
+    Qed.
 
   Lemma tau_invar_prop_subst_aux : forall A (a : A) (p : itree Void A -> Prop) (t t' : itree Void A), tau_invar Void A p ->
                                is_val A a t /\ is_val A a t' -> (p t -> p t').
@@ -91,11 +185,23 @@ Section PureITree.
     - apply IHHt. apply H. auto.
   Qed.
 
+  Lemma tau_invar_prop_subst_aux_eutt : forall A (a : A) (p : itree Void A -> Prop) (t t' : itree Void A), resp_eutt Void A p ->
+                                     is_val_eutt A a t /\ is_val_eutt A a t' -> (p t -> p t').
+    Proof.
+      intros. destruct H0 as [Ht Ht'].
+      unfold is_val_eutt in *. rewrite <- Ht in Ht'. eapply H; try eassumption.
+    Qed.
   Lemma tau_invar_prop_subst : forall A (a : A) (p : itree Void A -> Prop) (t t' : itree Void A), tau_invar Void A p ->
                                is_val A a t /\ is_val A a t' -> (p t <-> p t').
     Proof.
       split; intros; eapply tau_invar_prop_subst_aux; eauto.
       destruct H0. split; eauto.
+    Qed.
+
+  Lemma tau_invar_prop_subst_eutt : forall A (a : A) (p : itree Void A -> Prop) (t t' : itree Void A), resp_eutt Void A p ->
+                                     is_val_eutt A a t /\ is_val_eutt A a t' -> (p t <-> p t').
+    Proof.
+      split; intros; eapply tau_invar_prop_subst_aux_eutt; eauto. split; destruct H0; eauto.
     Qed.
 
 
@@ -106,50 +212,79 @@ Section PureITree.
     - pinversion H. subst. auto.
   Qed.
 
-  Lemma is_val_div : forall A (t : itree Void A), ~(exists a, is_val A a t) -> divergence t.
-    Proof.
-      intros. pcofix CIH. pfold.      -
-      destruct (observe t).
-      Admitted.
+  Ltac dest_void := match goal with [ E : Void ?A  |- _ ]=> destruct E end.  
 
-  Lemma is_val_or_div : forall A (t : itree Void A), (exists a, is_val A a t) \/ divergence t.
+  Lemma divergence_resp_eutt : forall A, resp_eutt Void A divergence.
     Proof.
-      intros.
-      destruct (classic (exists a, is_val A a t)); auto.
-      right. apply is_val_div. auto.
+      intro A. intro. intro.  intro. split.
+      - generalize dependent t2. generalize dependent t1. pcofix CIH.
+        intros. assert (Ht1 : divergence t1). auto. pfold. punfold H1. unfold divergence_ in *.
+        destruct (observe t1) eqn : Heqt1; destruct (observe t2) eqn : Heqt2; try dest_void; try inv_div_ret.
+        + specialize (itree_eta t2) as H. rewrite Heqt2 in H.
+          rewrite H in H0. rewrite H0 in Ht1. pinversion Ht1.
+        + constructor. inversion H1; subst. right. eapply CIH with (t1 := t1); eauto.
+          clear H2 H1. rewrite H0. clear Heqt1.  specialize (itree_eta t2) as H. rewrite Heqt2 in H.
+          rewrite <- (tau_eutt t0). rewrite H. reflexivity.
+      - generalize dependent t2. generalize dependent t1. pcofix CIH.
+        intros. assert (Ht2: divergence t2). auto. pfold. punfold H1. unfold divergence_ in *.
+        destruct (observe t1) eqn : Heqt1; destruct (observe t2) eqn : Heqt2; try dest_void; try inv_div_ret.
+        + specialize (itree_eta t1) as H. rewrite Heqt1 in H. rewrite H in H0.
+          rewrite <- H0 in Ht2. pinversion Ht2.
+        + constructor. inversion H1; subst. right. eapply CIH with (t2 := t2); eauto.
+          rewrite <- H0. clear H1 H2 Heqt2. specialize (itree_eta t1 ) as H. rewrite Heqt1 in H.
+          rewrite <- (tau_eutt t). rewrite H. reflexivity.
+  Qed.
+
+  Lemma divergence_resp_eutt' : forall A, resp_eutt Void A divergence.
+  Proof.
+    intros. unfold resp_eutt. intros. rewrite H. tauto.
+  Qed.
+
+  Lemma no_val_div : forall A , tau_invar Void A (fun t => ~exists a, is_val A a t).
+    Proof.
+      intros. split; intros; intro Hcontra.
+      - apply H. destruct Hcontra as [a Ha]. exists a. inv Ha. auto.
+      - apply H. destruct Hcontra as [a Ha]. exists a. constructor. auto.
     Qed.
 
-  (* maybe specifications only take tau invariant propositions  *)
+  Lemma eutt_reta_or_div_aux : forall A (t : itree Void A), ~(exists a, ret a ≈ t) -> divergence t.
+    Proof.
+      intro A. pcofix CIH. pfold. unfold divergence_.  intros. destruct (observe t) eqn : Heqt.
+      - exfalso. specialize (itree_eta t) as H. rewrite Heqt in H. apply H0.
+         exists r0. rewrite H. reflexivity.
+       - constructor. right. eapply CIH; eauto. intro. apply H0.
+         destruct H as [a Ha]. exists a. specialize (itree_eta t) as Ht. rewrite Heqt in Ht.
+         rewrite Ht. rewrite tau_eutt. auto.
+       - destruct e.
+    Qed.
 
-  Hint Constructors is_val.
-(*fails some monad laws if w does not admit any finite trees, some of these variables might have the wrong
-  scope *)
-  (* fun t => (exists a, is_val A a t /\ w t /\ f a p Hp) \/ (divergence t /\ w divergence)  *)
-(* should bind preserve infiniteness? *)
-  CoFixpoint spin {A : Type} : itree Void A := Tau spin.
+  Lemma eutt_reta_or_div : forall A (t : itree Void A), (exists a, ret a ≈ t) \/ (divergence t).
+    Proof.
+      intros A t.  specialize (classic (exists a, ret a ≈ t) ) as Hlem. destruct Hlem; auto.
+      right. apply eutt_reta_or_div_aux. auto.
+    Qed.
 
-  Lemma bind_pred_tau_invar : forall A B (f : A -> _PureITreeSpec B) 
-                                     (p : itree Void B -> Prop) (Hp : tau_invar Void B p), 
-      tau_invar Void A (fun (t : itree Void A) => (exists a, is_val A a t /\ f a p Hp) \/ 
+
+  Lemma bind_pred_resp_eutt : forall A B (f : A -> _PureITreeSpec B)
+                                     (p : itree Void B -> Prop) (Hp : resp_eutt Void B p),
+      resp_eutt Void A (fun (t : itree Void A) => (exists a, ret a ≈ t /\ f a p Hp) \/ 
                                                   (divergence t /\ p spin)).
   Proof.
-    intros. unfold tau_invar in *. split; intros.
-    - destruct H.
-      + left. destruct H as [a [Hvala Hfa] ]. exists a; split; auto.
-      + destruct H. right. split; auto. apply divergence_tau_invar in H. auto.
-    - destruct H.
-      + left. destruct H as [a [Hvala Hfa] ]. exists a; split; auto. inv Hvala. auto.
-      + destruct H. apply divergence_tau_invar in H. tauto.
+    intros. intros t1 t2 Heutt. split; intros; destruct H.
+    - destruct H as [ a [Hta Hfa] ]. left. exists a. rewrite Hta. auto.
+    - rewrite Heutt in H. auto.
+    - left. destruct H as [ a [Hta Hfa] ]. exists a. rewrite Hta. symmetry in Heutt. auto.
+    - rewrite <- Heutt in H. auto.
   Qed.
 
   
   (*intuitively, you have two choices, prove the tree evaluates to a and prove f a p,
     or prove t is infinite and prove that the infinite predicate is in w*)
   Definition _bindpi A B (w : _PureITreeSpec A) (f : A -> _PureITreeSpec B) :=
-    fun (p : itree Void B -> Prop) (Hp : tau_invar Void B p) =>
-      w (fun (t : itree Void A) => (exists a, is_val A a t /\ f a p Hp) \/ 
+    fun (p : itree Void B -> Prop) (Hp : resp_eutt Void B p) =>
+      w (fun (t : itree Void A) => (exists a, ret a ≈ t /\ f a p Hp) \/ 
                                    (divergence t /\  p spin ))
-  (bind_pred_tau_invar A B f p Hp).
+  (bind_pred_resp_eutt A B f p Hp).
 (* replace   *)
 
 
@@ -157,13 +292,13 @@ Section PureITree.
       monotonici A w -> (forall a, monotonici B (f a)) -> monotonici B (_bindpi A B w f).
   Proof.
     unfold monotonici. intros. unfold _bindpi in *.
-    set (fun t p0 Hp0 => (exists a, is_val A a t /\ f a p0 Hp0)\/ (divergence t /\ p spin))  as fp.
+    set (fun (t : itree Void A) p0 Hp0 => (exists a, ret a ≈ t /\ f a p0 Hp0)\/ (divergence t /\ p spin))  as fp.
     enough (forall t, fp t p Hp -> fp t p' Hp').
     - eapply H with (p := fun t => fp t p Hp).
-      + intros. subst. apply H3 in H4. 
+      + intros.  apply H3 in H4. 
         unfold fp in H4. destruct H4; auto.
-        destruct H4. right. split; auto.
-   + apply H2.
+        destruct H4. right. auto.
+      + apply H2.
     - unfold fp. intros. destruct H3; auto. left.
       intros. destruct H3 as [a [Hvala Hfa] ].
       exists a. split; auto.
@@ -188,7 +323,7 @@ Section PureITree.
 
 
   Global Instance PureITreeSpecEq : EqM PureITreeSpec :=
-    fun A w1 w2 => forall (p : itree Void A -> Prop) (Hp : tau_invar Void A p), proj1_sig w1 p Hp <-> proj1_sig w2 p Hp.
+    fun A w1 w2 => forall (p : itree Void A -> Prop) (Hp : resp_eutt Void A p), proj1_sig w1 p Hp <-> proj1_sig w2 p Hp.
 
 
   Lemma ret_not_div : forall (A : Type) (E : Type -> Type) (a : A), ~ (@divergence E A (ret a)).
@@ -196,22 +331,29 @@ Section PureITree.
       intros. intro Hcontra. pinversion Hcontra.
     Qed.
 
-  Lemma bindpi_retpi : forall A B (f : A -> PureITreeSpec B) (a : A), 
+  Lemma inv_ret : forall (A : Type) (E : Type -> Type) (a b : A),
+        @eutt E A A eq (ret a) (ret b) -> a = b.
+    Proof. 
+      intros. pinversion H; subst. auto.
+    Qed.
+ 
+  Lemma retpi_bindpi : forall A B (f : A -> PureITreeSpec B) (a : A), 
       bind (ret a) f ≈ f a.
     Proof.
       intros. split.
       - cbn. unfold _bindpi. unfold _retpi. intros. 
         destruct H.
-        + destruct H as [a0 [Hvala0 Hfa0] ]. inversion Hvala0. subst. auto.
-        + exfalso. destruct H. eapply ret_not_div. eauto. 
+        + destruct H as [a0 [Hvala0 Hfa0] ].
+          apply inv_ret in Hvala0. subst. auto.
+        + exfalso. destruct H. eapply ret_not_div. eauto.
       - simpl. destruct (f a) as [fa Hfa] eqn : Heq. simpl. intros.
         left. exists a. split; auto.
-        + constructor.
+        + reflexivity.
         + rewrite Heq. auto.
     Qed.
 
     
-  Lemma retpi_bindpi : forall A (w : PureITreeSpec A), bind w (fun x => ret x) ≈ w.
+  Lemma bindpi_retpi : forall A (w : PureITreeSpec A), bind w (fun x => ret x) ≈ w.
   Proof.
     intros. destruct w as [ w Hw]. split.
     - intros. simpl in *. unfold _bindpi in H.
@@ -220,49 +362,42 @@ Section PureITree.
       2: apply H.
       intros. destruct H0.
       + destruct H0 as [a [ Hvala Hpa]  ].
-        induction Hvala; auto. apply Hp in IHHvala. auto.
-      + destruct H0. (* this is proven by inf taus being obs equivalent, that should be provable  *) admit.
+        eapply Hp; eauto. symmetry. auto.
+      + destruct H0. apply div_spin_eutt in H0. eapply Hp; eauto.
     - simpl. intros. unfold _bindpi.
-      eapply Hw. 2: apply H. intros.
-      destruct (is_val_or_div A i').
-      + left. destruct H1 as [ a Ha ]. exists a. split; auto.
-        unfold _retpi. eapply tau_invar_prop_subst; eauto.
-        split. constructor. auto.
-      + right. split; auto. (* same as the other unsolved case*)
-   Admitted.    
-
+      eapply Hw. 2: apply H. intros. unfold _retpi.
+      specialize (eutt_reta_or_div A i') as Hor. destruct Hor.
+      + destruct H1 as [a Ha]. left. exists a. split; auto. eapply Hp; eauto.
+      + right. split; auto. specialize (div_spin_eutt A i' H1) as H2. eapply Hp; eauto. symmetry. auto.
+   Qed.
   Lemma bindpi_bindpi : forall (A B C : Type) (w : PureITreeSpec A) 
                                (f : A -> PureITreeSpec B) (g : B -> PureITreeSpec C),
       bind (bind w f) g ≈ bind w (fun a => bind (f a) g).
     Proof.
-      intros. destruct w as [w Hw]. split; simpl.
-      - intros. eapply Hw; try apply H.
-        intros. destruct H0; try destruct H0.
-        + destruct H0. simpl in *.
-          left. exists x. split; auto. unfold bindpi. destruct (f x) as [fx Hfx].
-          simpl in *. unfold _bindpi.
-          
-          eapply Hfx; try apply H1.
-          intros. destruct H2.
-          * destruct H2 as [b [Hvalb Hgb ] ].
-            left. exists b. auto.
-          * destruct H2. right. split; auto.
-        + unfold _bindpi in H.(* eapply Hw.
-
-          destruct H1. simpl in *.
-          * 
-      *)
-
-  Admitted.
+      intros. destruct w as [w Hw]. simpl. split; intros.
+      - simpl in *. eapply Hw; try apply H. intros t0. intros. destruct H0.
+        + destruct H0 as [a [Hreta Hfa] ].
+          left. exists a. split; auto. destruct (f a) as [wfa Hwfa]. simpl in *.
+          eapply Hwfa; try (apply Hfa). intros t1. intros. destruct H0; auto.
+        + destruct H0. destruct H1.
+          * destruct H1 as [b [Hretb Hgb ]  ]. exfalso. specialize (ret_not_div B Void b) as Hndiv.
+            rewrite Hretb in Hndiv. apply Hndiv. apply spin_div.
+          *  right. destruct H1. auto.
+      - simpl in *. eapply Hw; try apply H. intros t0. intros. destruct H0.
+        +  destruct H0 as [a [Hreta Hfa] ]. left. exists a. split; auto.
+           destruct (f a) as [wfa Hwfa]. simpl in *. eapply Hwfa; try (apply Hfa). intros t1. intros.
+           destruct H0; auto.
+        + destruct H0. right. split; auto. right. split; auto. apply spin_div.
+    Qed.
 
 
   Global Instance PureItreeSpecLaws : MonadLaws PureITreeSpec.
   Proof.
     constructor.
-    - intros A B f a. cbv. intros. destruct (f a) as [w Hw] eqn : Heq. split; intros.
-      + unfold monotonici in *. eapply Hw.
-        * intros. admit.
-        * Abort.
+    - apply retpi_bindpi.
+    - apply bindpi_retpi.
+    - apply bindpi_bindpi.
+  Qed.  
 
   (* does this satisfy the monad laws? is it unique in some sense, if not what are the implications of
    this choice*)
@@ -283,7 +418,8 @@ Section StateITree.
   Definition StateITree A := itree (stateE S) A.
 
   Definition _StateITreeSpec A := (itree Void (A * S) -> Prop) -> S -> Prop.
-
+End StateITree.
+(*
   Definition _interpStateSpec : (stateE S) ~> (_StateSpec S) :=
     fun _ (ev : stateE S _) =>
       match ev with
@@ -305,7 +441,7 @@ Section StateITree.
   Lemma retis_monot : forall A a, monotonicis A (_retis A a).
   Proof.
     unfold monotonicis. intros. unfold _retis in *. auto.
-  Qed.
+  Qed. *)
 (* bind I think needs some coinduction, I'll leave it out for now
   Definition _bindis A B (m : _StateItreeSpec A) (f : A -> _StateItreeSpec B) :=
     fun p s => m (fun '(i,s') =>  ) s
@@ -316,7 +452,7 @@ Section StateITree.
     problem is the first case doesn't terminate, need more info on coinduction from Steve maybe?
 *)
 
-
+(*
 
   Definition StateITreeSpec A := {w : _StateITreeSpec A | monotonicis _ w}.
 
@@ -344,4 +480,5 @@ End StateITree.
   
 
   CoInductive t :=.
+*)
 *)
